theories/Block/vst/verif/certicoq_block__header_get_ptr.v
@@ -1,0 +1,17 @@
+From VST Require Import floyd.proofauto.
+
+From CertiCoq Require Import Block.vst.ast.ast.
+From CertiCoq Require Import Block.vst.clightgen.block.
+From CertiCoq Require Import Block.vst.cmodel.certicoq_block_header.
+From CertiCoq Require Import Block.vst.cmodel.certicoq_block.
+From CertiCoq Require Import Block.vst.spec.spec.
+
+Lemma body: semax_body Vprog ASI f_certicoq_block__header_get_ptr certicoq_block__header_get_ptr_spec.
+Proof.
+  start_function.
+  forward.
+  {
+    entailer!.
+    destruct block ; now try contradiction.
+  }
+Qed.
